RBT_height.thy
@@ -6,7 +6,8 @@ begin
    than using the built-in function for converting lists into sets. *)
 
 typedef (overloaded) 'a sdlist = "{xs :: ('a :: ccompare) list.
-  case ID CCOMPARE('a) of None \<Rightarrow> xs = [] | Some _ \<Rightarrow> linorder.sorted cless_eq xs \<and> distinct xs}"
+  case ID CCOMPARE('a) of None \<Rightarrow> xs = []
+  | Some c \<Rightarrow> linorder.sorted (le_of_comp c) xs \<and> distinct xs}"
   by (auto intro!: exI[of _ "[]"] split: option.splits)
      (metis keys_eq_Nil_iff sorted_RBT_Set_keys)
 
@@ -15,8 +16,8 @@ setup_lifting type_definition_sdlist
 lemma sset_rbt:
   fixes xs :: "('a :: ccompare) list"
     and c :: "'a comparator"
-  assumes assms: "ID ccompare = Some c" "linorder.sorted cless_eq xs" "distinct xs"
-  shows "ord.is_rbt cless (rbtreeify (map (\<lambda>x. (x, ())) xs))"
+  assumes assms: "ID ccompare = Some c" "linorder.sorted (le_of_comp c) xs" "distinct xs"
+  shows "ord.is_rbt (lt_of_comp c) (rbtreeify (map (\<lambda>x. (x, ())) xs))"
   using assms linorder.is_rbt_rbtreeify[OF ID_ccompare[OF assms(1)], of "map (\<lambda>x. (x, ())) xs"]
   by (auto simp: comp_def)
 
@@ -25,16 +26,11 @@ lift_definition sset :: "('a :: ccompare) sdlist \<Rightarrow> 'a set_rbt" is
   using sset_rbt
   by fastforce
 
-lemma Rep_sdlist_keys:
-  fixes xs :: "('a :: ccompare) sdlist"
-  shows "Rep_sdlist xs = RBT_Set2.keys (sset xs)"
-  by transfer (auto simp: RBT_Impl.keys_def comp_def)
-
 lemma rbt_comp_lookup_iff_in_set:
   fixes x :: "'a :: ccompare"
     and xs :: "'a list"
     and c :: "'a comparator"
-  assumes "ID ccompare = Some c" "linorder.sorted cless_eq xs" "distinct xs"
+  assumes "ID ccompare = Some c" "linorder.sorted (le_of_comp c) xs" "distinct xs"
   shows "rbt_comp_lookup ccomp (rbtreeify (map (\<lambda>x. (x, ())) xs)) x = Some () \<longleftrightarrow> x \<in> set xs"
   using linorder.rbt_lookup_rbtreeify[OF ID_ccompare[OF assms(1)], of "map (\<lambda>x. (x, ())) xs"]
       assms(2,3)
@@ -49,37 +45,50 @@ lemma RBT_set_sset:
   using rbt_comp_lookup_iff_in_set
   by (fastforce simp: rbtreeify_def split: option.splits)
 
-lemma linorder_sorted_upt: "linorder.sorted (le_of_comp compare) [n..<n']"
-proof -
-  define c :: "nat comparator" where "c = compare"
-  have cl: "class.linorder (le_of_comp c) (lt_of_comp c)"
-    by (auto simp: c_def ID_ccompare ID_Some ccompare_nat_def)
-  show ?thesis
-    using linorder.sorted_sorted_wrt[OF cl] sorted_wrt_mono_rel[OF _ sorted_wrt_upt]
-    by (auto simp: c_def ord_defs(1))
-qed
+lemma quicksort_conv_sort_key:
+  fixes f :: "'b \<Rightarrow> 'a :: ccompare"
+  assumes "ID (ccompare :: 'a comparator option) = Some c"
+  shows "ord.quicksort (lt_of_comp c) xs = linorder.sort_key (le_of_comp c) (\<lambda>x. x) xs"
+  by (rule linorder.quicksort_conv_sort[OF ID_ccompare[OF assms]])
 
-lift_definition upt_sdlist :: "nat \<Rightarrow> nat \<Rightarrow> nat sdlist" is upt
-  using linorder_sorted_upt
-  by (auto simp: ID_Some ccompare_nat_def split: option.splits)
+context linorder
+begin
 
-definition nat_set_upt :: "nat \<Rightarrow> nat \<Rightarrow> nat set" where
-  "nat_set_upt i j = {i..<j}"
+lemma distinct_remdups_adj: "sorted xs \<Longrightarrow> distinct (remdups_adj xs)"
+  by (induction xs rule: remdups_adj.induct) auto
 
-lemma nat_set_upt_code[code]: "nat_set_upt i j = RBT_set (sset (upt_sdlist i j))"
-  by (auto simp: nat_set_upt_def RBT_set_sset upt_sdlist.rep_eq)
+end
 
-definition run :: "nat \<Rightarrow> nat \<Rightarrow> nat set" where
-  "run i l = {i * l ..< Suc i * l}"
+lift_definition sdlist_of_list :: "('a :: ccompare) list \<Rightarrow> 'a sdlist" is
+  "\<lambda>xs :: 'a list. case ID CCOMPARE('a) of None \<Rightarrow> []
+  | Some c \<Rightarrow> remdups_adj (ord.quicksort (lt_of_comp c) xs)"
+  using linorder.sorted_remdups_adj[OF ID_ccompare linorder.sorted_sort[OF ID_ccompare]]
+  using linorder.distinct_remdups_adj[OF ID_ccompare linorder.sorted_sort[OF ID_ccompare]]
+  using quicksort_conv_sort_key
+  by (fastforce split: option.splits)
 
-lemma run_code[code]: "run i l = nat_set_upt (i * l) (Suc i * l)"
-  by (auto simp: run_def nat_set_upt_def)
+lemma set_sdlist_of_list:
+  fixes xs :: "('a :: ccompare) list"
+    and c :: "'a comparator"
+  assumes assms: "ID ccompare = Some c"
+  shows "set (Rep_sdlist (sdlist_of_list xs)) = set xs"
+  using assms
+  apply transfer
+  using linorder.set_sort[OF ID_ccompare] quicksort_conv_sort_key
+  by fastforce
 
-definition compare_height_rbt :: "(nat, unit) mapping_rbt \<Rightarrow> (nat, unit) mapping_rbt \<Rightarrow>
-  RBT_Impl.compare" where
-  "compare_height_rbt t1 t2 =
-    RBT_Impl.compare_height (RBT_Mapping2.impl_of t1) (RBT_Mapping2.impl_of t1)
-    (RBT_Mapping2.impl_of t2) (RBT_Mapping2.impl_of t2)"
+lemma set_code:
+  fixes xs :: "('a :: ccompare) list"
+  shows "set xs = (case ID CCOMPARE('a) of None \<Rightarrow> Code.abort (STR ''set: ccompare = None'')
+    (\<lambda>_. set xs)
+  | Some _ \<Rightarrow> RBT_set (sset (sdlist_of_list xs)))"
+  by (auto simp: RBT_set_sset set_sdlist_of_list split: option.splits)
+
+definition nat_set_upt :: "nat \<Rightarrow> nat \<Rightarrow> nat list" where
+  "nat_set_upt i j = [i..<j]"
+
+definition nat_set :: "nat list \<Rightarrow> nat set" where
+  "nat_set = set"
 
 definition un_nat_set :: "nat set \<Rightarrow> nat set \<Rightarrow> nat set" where
   "un_nat_set X Y = X \<union> Y"
@@ -87,9 +96,18 @@ definition un_nat_set :: "nat set \<Rightarrow> nat set \<Rightarrow> nat set" w
 definition int_nat_set :: "nat set \<Rightarrow> nat set \<Rightarrow> nat set" where
   "int_nat_set X Y = X \<inter> Y"
 
-export_code run compare_height_rbt un_nat_set int_nat_set
-  nat_of_integer integer_of_nat RBT_set RBT_Impl.EQ
+definition compare_height_rbt :: "(nat, unit) mapping_rbt \<Rightarrow> (nat, unit) mapping_rbt \<Rightarrow>
+  RBT_Impl.compare" where
+  "compare_height_rbt t1 t2 =
+    RBT_Impl.compare_height (RBT_Mapping2.impl_of t1) (RBT_Mapping2.impl_of t1)
+    (RBT_Mapping2.impl_of t2) (RBT_Mapping2.impl_of t2)"
+
+export_code nat_set_upt nat_set un_nat_set int_nat_set
+  nat_of_integer integer_of_nat compare_height_rbt RBT_set RBT_Impl.EQ
   in OCaml module_name RBT_height file_prefix "RBT_height_old"
+
+declare Set_Impl.set_code[code del]
+declare set_code[code]
 
 declare Set_union_code(1)[code del]
 declare rbt_union_code[code]
@@ -100,8 +118,8 @@ declare rbt_inter_code[code]
 declare Set_minus_code[code del]
 declare rbt_minus_code[code]
 
-export_code run compare_height_rbt un_nat_set int_nat_set
-  nat_of_integer integer_of_nat RBT_set RBT_Impl.EQ
+export_code nat_set_upt nat_set un_nat_set int_nat_set
+  nat_of_integer integer_of_nat compare_height_rbt RBT_set RBT_Impl.EQ
   in OCaml module_name RBT_height file_prefix "RBT_height_opt"
 
 end
